wow, a monadic profiler

src/tidy/monad_chain.lean
@@ -1,3 +1,6 @@
+import .if_then_else
+import .tidy
+
 universe variables u v w
 
 meta class tactical_monad (m : Type u → Type v) extends monad_fail m, has_orelse m :=
@@ -10,10 +13,6 @@ meta def fail {α : Type u} { m : Type u → Type v } [tactical_monad m] {β : T
 meta instance lift_tactic_coe (α : Type u) (m : Type u → Type v) [tactical_monad m]: has_coe (tactic α) (m α) :=
 ⟨ tactical_monad.lift _ ⟩
 
-meta def if_then_else { α β : Type } { m : Type → Type } [monad m] [has_orelse m] ( i : m α ) ( t e : m β ) : m β :=
-do r ← (i >> pure tt) <|> pure ff,
-   if r then do t else do e
-
 private meta structure chain_progress ( α : Type ) ( m : Type → Type ) [monad m] :=
   ( iteration_limit   : nat )
   ( results           : list α )
@@ -23,17 +22,95 @@ open nat tactic
 
 private meta def chain' { α : Type } { m : Type → Type } [tactical_monad m] ( tactics : list (m α) ) 
     : chain_progress α m → m (list α)
-| ⟨ 0, _, _ ⟩                  := fail ""
-| ⟨ _, results, [] ⟩           := (pure results) 
+| ⟨ 0     , _      , _       ⟩ := fail "chain iteration limit exceeded"
+| ⟨ _     , results, []      ⟩ := pure results
 | ⟨ succ n, results, t :: ts ⟩ := if_then_else done
                                    (pure results)
-                                   (pure [])
+                                   (dependent_if_then_else t 
+                                      (λ result, (chain' ⟨ n, result :: results, tactics ⟩ ))
+                                      (chain' ⟨ succ n, results, ts ⟩)
+)
 
 meta instance trivial_tactical_monad : tactical_monad tactic := {
   interaction_monad.monad with
-  fail := sorry,
-  orelse := sorry,
-  lift := λ { α : Type }, id
+  fail   := λ { α : Type }, tactic.fail,
+  orelse := λ { α : Type }, interaction_monad_orelse,
+  lift   := λ { α : Type }, id
 }
 
 meta def skip2 : tactic ( list unit ) := let tactics := [skip, skip] in chain' tactics ⟨ 0, [], tactics ⟩
+
+structure profiling_state :=
+  ( invocations : nat )
+
+meta def stateful_tactic (β : Type) (α : Type) := β → tactic ((interaction_monad.result tactic_state α) × β)
+
+meta def profiling_tactic := stateful_tactic profiling_state
+
+meta def tactic_pure { α : Type } ( a : α ) : tactic α := pure a
+
+meta def unreachable {α : Sort u} : α := undefined_core "unreachable"
+
+meta instance profiling_tactical_monad : tactical_monad profiling_tactic := { 
+  pure   := λ { α : Type } ( a : α ) ( s : profiling_state ) ( ts : tactic_state ),
+              match ((tactic_pure a) ts) with
+              | (result.success a ts')         := result.success (result.success a ts', s) ts'
+              | (result.exception msg pos ts') := unreachable
+              end,
+  bind   := λ { α β : Type } ( t : profiling_tactic α ) ( f : α → profiling_tactic β ) ( s : profiling_state ) ( ts : tactic_state ),
+              match (t s ts) with
+              | (result.success r ts')         := match r with 
+                                                  | (result.success a ts',         ps') := f a ps' ts'
+                                                  | (result.exception msg pos ts', ps') := result.success (result.exception msg pos ts', ps') ts'
+                                                  end
+              | (result.exception msg pos ts') := unreachable
+              end,
+  fail   := λ { α : Type } (msg : string) ( s : profiling_state ), (do @tactic.fail _ string _ msg),
+  orelse := λ { α : Type } ( t : profiling_tactic α ) ( t' : profiling_tactic α ) ( s : profiling_state ) ( ts : tactic_state ),
+              match (t s ts) with
+              | (result.success r ts')         := match r with 
+                                                  | (result.success a ts',         ps') := (result.success r ts')
+                                                  | (result.exception msg pos ts', ps') := t' ps' ts'
+                                                  end
+              | (result.exception msg pos ts') := unreachable
+              end,
+  lift   := λ { α : Type } ( t : tactic α ) ( s : profiling_state ) ( ts : tactic_state ),
+              match (t ts) with
+              | (result.success a ts')         := result.success (result.success a ts', ⟨ s.invocations + 1 ⟩ ) ts'
+              | (result.exception msg pos ts') := result.success (result.exception msg pos ts', ⟨ s.invocations + 1 ⟩) ts'
+              end,
+  id_map     := begin tidy, end,
+  pure_bind  := undefined,
+  bind_assoc := undefined,            
+}
+
+meta def empty_profiling_state : profiling_state := ⟨ 0 ⟩ 
+
+meta def profiling { α : Type } ( t : profiling_tactic α ) : tactic (ℕ × α) :=
+do r ← t empty_profiling_state,
+   trace r.2.invocations,
+   match r.1 with 
+   | result.success a ts := pure (r.2.invocations, a)
+   | result.exception msg pos ts := match msg with
+                                    | (some m) := tactic.fail ( m () )
+                                    | none     := tactic.failed
+                                    end
+   end
+
+lemma f : true :=
+begin
+profiling $ skip >> skip,             -- 2
+profiling $ skip >> skip >> skip,     -- 3
+success_if_fail { profiling $ done }, -- 1
+
+profiling $ skip <|> done,            -- 1
+profiling $ done <|> skip,            -- 2
+
+profiling $ (skip <|> done) >> skip, -- 2
+
+profiling $ done <|> done <|> skip, -- 3
+
+success_if_fail { profiling $ done <|> done }, -- 2
+
+triv
+end
