src/tidy/monad_chain.1.lean
@@ -1,0 +1,135 @@
+import .if_then_else
+import .tidy
+
+universe variables u v w
+
+meta class tactical_monad (m : Type u → Type v) extends monad_fail m, has_orelse m :=
+  ( lift : Π { α : Type u }, tactic α → m α )
+
+meta def failed {α : Type u} { m : Type u → Type v } [tactical_monad m]: m α := monad_fail.fail m ""
+meta def fail {α : Type u} { m : Type u → Type v } [tactical_monad m] {β : Type u} [has_to_format β] (msg : β) : m α :=
+  monad_fail.fail m (to_fmt msg).to_string
+
+meta instance lift_tactic_coe (α : Type u) (m : Type u → Type v) [tactical_monad m]: has_coe (tactic α) (m α) :=
+⟨ tactical_monad.lift _ ⟩
+
+
+private meta structure chain_progress ( α : Type ) ( m : Type → Type ) [monad m] :=
+  ( iteration_limit   : nat )
+  ( results           : list α )
+  ( remaining_tactics : list (m α) )
+
+open nat tactic
+
+private meta def chain' { α : Type } { m : Type → Type } [tactical_monad m] ( tactics : list (m α) ) 
+    : chain_progress α m → m (list α)
+| ⟨ 0     , _      , _       ⟩ := fail "chain iteration limit exceeded"
+| ⟨ _     , results, []      ⟩ := pure results
+| ⟨ succ n, results, t :: ts ⟩ := if_then_else done
+                                   (pure results)
+                                   (dependent_if_then_else t 
+                                      (λ result, (chain' ⟨ n, result :: results, tactics ⟩ ))
+                                      (chain' ⟨ succ n, results, ts ⟩)
+)
+
+meta instance trivial_tactical_monad : tactical_monad tactic := {
+  interaction_monad.monad with
+  fail   := λ { α : Type }, tactic.fail,
+  orelse := λ { α : Type }, interaction_monad_orelse,
+  lift   := λ { α : Type }, id
+}
+
+meta def skip2 : tactic ( list unit ) := let tactics := [skip, skip] in chain' tactics ⟨ 0, [], tactics ⟩
+
+structure profiling_state :=
+  ( invocations : nat )
+
+meta def stateful_tactic (β : Type) (α : Type) := interaction_monad (tactic_state × β) α
+
+meta def profiling_tactic := stateful_tactic profiling_state
+
+meta def tactic_pure { α : Type } ( a : α ) : tactic α := pure a
+meta def tactic_state_pure { α : Type } ( a : α ) ( ts : tactic_state ) : tactic_state :=
+begin
+  have p := tactic_pure a ts,
+  induction p with _ ts' _ _ ts'',
+  exact ts',
+  exact ts''
+end
+meta def tactic_pure_lemma { α : Type } ( a : α ) ( ts : tactic_state ) : tactic_pure a ts = result.success a (tactic_state_pure a ts) :=
+begin
+  dunfold tactic_state_pure,
+  dunfold tactic_pure,
+  dunfold pure,
+  dunfold tactic,
+  dunfold interaction_monad,
+  dunfold has_pure.pure,
+  dunfold interaction_monad_return,
+  dsimp,
+  refl  
+end
+
+meta def unreachable {α : Sort u} : α := undefined_core "unreachable"
+
+meta instance profiling_tactical_monad : tactical_monad profiling_tactic := { 
+  pure   := λ { α : Type } ( a : α ) ( s : tactic_state × profiling_state ), 
+              result.success a (tactic_state_pure a s.1, ⟨ s.2.invocations + 1 ⟩),
+  bind   := λ { α β : Type } ( t : profiling_tactic α ) ( f : α → profiling_tactic β ) ( s : tactic_state × profiling_state ), 
+              match (t s) with
+              | result.success a s' := f a s'
+              | result.exception pos msg s' := result.exception pos msg s'
+              end,
+  lift   := λ { α : Type } ( t : tactic α ) ( s : tactic_state × profiling_state ), 
+              match (t s.1) with
+              | result.success a s' := result.success a (s', ⟨ s.2.invocations + 1 ⟩ )
+              | result.exception pos msg s' := result.exception pos msg (s', ⟨ s.2.invocations + 1 ⟩ )
+              end,
+  fail   := λ { α : Type } (msg : string), begin admit end,
+  orelse := λ { α : Type } ( t₁ : profiling_tactic α ) ( t₂ : profiling_tactic α ) ( s : tactic_state × profiling_state ), 
+              match (t₁ s) with
+              | result.success a s' := result.success a s'
+              | result.exception pos msg s' := t₂ s'
+              end,
+  id_map     := undefined,
+  pure_bind  := undefined,
+  bind_assoc := undefined,            
+}
+
+meta def empty_profiling_state : profiling_state := ⟨ 0 ⟩ 
+
+meta def profiling
+  { α : Type } ( t : profiling_tactic α )
+  ( success_handler   : profiling_state → tactic unit := λ p, trace format!"success, with {p.invocations} invocations" ) 
+  ( exception_handler : profiling_state → tactic unit := λ p, trace format!"failed, with {p.invocations} invocations" ) 
+    : tactic (α × profiling_state) :=
+λ s, match t (s, empty_profiling_state) with
+     | result.success a ts         :=
+         match success_handler ts.2 ts.1 with
+         | result.success _ _             := result.success (a, ts.2) ts.1
+         | result.exception msg' pos' ts' := result.exception msg' pos' ts'  -- Ugh, an exception in the exception handler!
+         end        
+     | result.exception msg pos ts := 
+         match exception_handler ts.2 ts.1 with
+         | result.success _ _             := result.exception msg pos ts.1
+         | result.exception msg' pos' ts' := result.exception msg' pos' ts'  -- Ugh, an exception in the exception handler!
+         end
+     end 
+
+
+lemma f : true :=
+begin
+profiling $ skip >> skip,             -- 2
+profiling $ skip >> skip >> skip,     -- 3
+success_if_fail { profiling $ done }, -- 1
+
+profiling $ skip <|> done,            -- 1
+profiling $ done <|> skip,            -- 2
+
+profiling $ (skip <|> done) >> skip, -- 2
+
+profiling $ done <|> done <|> skip, -- 3
+
+success_if_fail { profiling $ done <|> done }, -- 2
+
+triv
+end
